Merge Hist in IOStar

seiostar/IOStar.fst
@@ -2,8 +2,6 @@ module IOStar
 
 open FStar.Tactics.V1
 
-include BaseTypes
-include Hist
 include Trace
 
 (** Computational Monad **)
@@ -34,15 +32,168 @@ let io_call (o:io_ops) (args:io_args o) : io (io_res o args) =
 let return = io_return
 let (let!@) = io_bind
 
-let op_wp (o:io_ops) (args:io_args o) : hist (io_res o args) =
+(** Specification monad **)
+
+(** The postcondition for an io computation is defined over the
+result (type: a) and local trace (type: list event).
+The local trace represents the events that happend during the
+computation. Local trace is in chronological order.
+
+We also have the history (type: list event) that represents the
+events that happend until the beginning of the io computation.
+The history is in reverse chronological order.
+
+At the end of an io computation, the local trace is
+reversed and appended to the history. **)
+
+type hist_post (h:history) a = lt:local_trace h -> r:a -> Type0
+type hist_pre = h:history -> Type0
+
+type hist0 a =
+  h:history -> hist_post h a -> Type0
+
+unfold
+let hist_post_ord (#h:history) (p1 p2:hist_post h 'a) = forall lt r. p1 lt r ==> p2 lt r
+
+unfold
+let hist_post_equiv (#h:history) (p1 p2:hist_post h 'a) =
+  hist_post_ord p1 p2 /\ hist_post_ord p2 p1
+
+unfold
+let hist_post_bind #h (m:hist_post h 'a) (k:(lt:local_trace h -> 'a -> hist_post (h++lt) 'b)) : hist_post h 'b =
+  fun lt b ->
+    exists a lta ltb. m lta a /\ lta@ltb == lt /\ k lta a ltb b
+
+unfold
+let hist_wp_monotonic (wp:hist0 'a) =
+  forall h (p1 p2:hist_post h 'a). (p1 `hist_post_ord` p2) ==>  (wp h p1 ==> wp h p2)
+
+type hist a = wp:(hist0 a){hist_wp_monotonic wp}
+
+let wp2p (wp:hist 'a) (h:history) : hist_post h 'a =
+  fun lt res -> forall p. wp h p ==> p lt res
+
+val hist_subcomp0 : #a:Type -> #p1:(a -> Type0) -> #p2:(a -> Type0) -> #_:unit{forall x. p1 x ==> p2 x} -> wp:hist (x:a{p1 x}) ->
+  (hist (x:a{p2 x}))
+let hist_subcomp0 #a #p1 #p2 #_ wp : (hist (x:a{p2 x})) =
+  let wp' : hist0 (x:a{p2 x}) = wp in
+  assert (forall h (post1:hist_post h (x:a{p2 x})) (post2:hist_post h (x:a{p2 x})). (hist_post_ord post1 post2 ==>  wp' h post1 ==> wp' h post2));
+  assert (hist_wp_monotonic #(x:a{p2 x}) wp');
+  wp'
+
+val hist_subcomp : #a:Type -> #p1:(a -> Type0) -> #p2:(a -> Type0) -> wp:hist (x:a{p1 x}) ->
+  Pure (hist (x:a{p2 x})) (requires (forall x. p1 x ==> p2 x)) (ensures (fun _ -> True))
+let hist_subcomp #a #p1 #p2 wp = hist_subcomp0 #a #p1 #p2 #() wp
+
+
+unfold
+let hist_return0 (x:'a) : hist0 'a =
+  fun _ p -> p [] x
+
+unfold
+let hist_return (x:'a) : hist 'a = hist_return0 x
+
+unfold
+let hist_post_shift (h:history) (p:hist_post h 'a) (lt:local_trace h) : hist_post (h++lt) 'a =
+  fun lt' r -> p (lt @ lt') r
+
+unfold
+let hist_post_bind'
+  (#a #b:Type)
+  (#h:history)
+  (kw : a -> hist b)
+  (p:hist_post h b) :
+  Tot (hist_post h a) =
+  fun lt r ->
+    kw r (h ++ lt) (hist_post_shift h p lt)
+
+unfold
+let hist_bind (#a #b:Type) (w : hist a) (kw : a -> hist b) : hist b =
+  fun h p -> w h (hist_post_bind' kw p)
+
+unfold
+let to_hist (#op:io_ops) (#args:io_args op) (pre:hist_pre) (post:(h:history -> io_res op args -> local_trace h -> Type0)) : hist (io_res op args)  =
+  fun h p -> pre h /\ (forall lt r. post h r lt ==> p lt r)
+
+let hist_call (o:io_ops) (args:io_args o) : hist (io_res o args) =
   to_hist
     (fun h -> io_pre h o args)
     (fun h res lt -> io_post h o args res /\ lt == [op_to_ev o args res])
 
+unfold
+let wp_lift_pure_hist0 (#a:Type u#a) (w : pure_wp a) : hist0 a =
+  FStar.Monotonic.Pure.elim_pure_wp_monotonicity_forall u#a ();
+  fun _ p -> w (p [])
+
+unfold
+let wp_lift_pure_hist (#a:Type u#a) (w : pure_wp a) : hist a =
+  FStar.Monotonic.Pure.elim_pure_wp_monotonicity_forall u#a ();
+  wp_lift_pure_hist0 w
+
+let lemma_wp_lift_pure_hist_implies_as_requires #a w :
+  Lemma (forall h (p:hist_post h a). wp_lift_pure_hist w h p ==> as_requires w) =
+    assert (forall h (p:hist_post h a) x. p [] x ==> True) ;
+    FStar.Monotonic.Pure.elim_pure_wp_monotonicity w ;
+    assert (forall h (p:hist_post h a). w (fun x -> p [] x) ==> w (fun _ -> True))
+
+unfold
+val (⊑) (#a : Type) : hist a -> hist a -> Type0
+let (⊑) wp1 wp2 = forall h p. wp2 h p ==> wp1 h p
+
+unfold
+val hist_equiv (#a : Type) : hist a -> hist a -> Type0
+let hist_equiv wp1 wp2 = forall h p. wp1 h p <==> wp2 h p
+
+unfold
+let hist_if_then_else (wp1 wp2:hist 'a) (b:bool) : hist 'a =
+  fun h p -> (b ==> wp1 h p) /\ ((~b) ==> wp2 h p)
+
+let lem_hist_bind_subset (#a #b:Type) (m m':hist a) (k k':a -> hist b) :
+  Lemma
+    (requires (m ⊑ m' /\ (forall x. k x ⊑ k' x)))
+    (ensures (hist_bind m k ⊑ hist_bind m' k')) = ()
+
+let lem_hist_bind_equiv (#a #b:Type) (m m':hist a) (k k':a -> hist b) :
+  Lemma
+    (requires (m `hist_equiv` m' /\ (forall x. k x `hist_equiv` k' x)))
+    (ensures (hist_bind m k `hist_equiv` hist_bind m' k')) = ()
+
+let lem_hist_equiv_reflexive #a (m:hist a) :
+  Lemma (m `hist_equiv` m) = ()
+
+let lem_hist_equiv_commutative #a (m m':hist a) :
+  Lemma (m `hist_equiv` m' ==> m' `hist_equiv` m) = ()
+
+module L = FStar.List.Tot
+
+let __list_assoc_l #a (l1 l2 l3 : list a) : Lemma (L.append l1 (l2 `L.append` l3) == (l1 `L.append` l2) `L.append` l3) = List.Tot.Properties.append_assoc l1 l2 l3
+let __helper #a (lt lt' : list a) : Lemma (L.rev_acc lt [] `L.append` L.rev_acc lt' [] == L.rev_acc (lt' `L.append` lt) []) = List.Tot.Properties.rev_append lt' lt
+let __iff_refl a : Lemma (a <==> a) = ()
+
+let lemma_hist_bind_associativity #a #b #c (w1:hist a) (w2:a -> hist b) (w3: b -> hist c) :
+  Lemma (hist_bind w1 (fun r1 -> hist_bind (w2 r1) w3) `hist_equiv` hist_bind (hist_bind w1 w2) w3)
+  =
+  let lhs = hist_bind w1 (fun r1 -> hist_bind (w2 r1) w3) in
+  let rhs = hist_bind (hist_bind w1 w2) w3 in
+  let pw (h : history) (p : hist_post h c) : Lemma (lhs h p <==> rhs h p) =
+    assert (lhs h p <==> rhs h p) by begin
+      unfold_def (`hist_bind);
+      norm [];
+      l_to_r [`__list_assoc_l];
+      l_to_r [`__helper];
+      mapply (`__iff_refl)
+    end
+  in
+  Classical.forall_intro_2 pw
+
+(** Semantics of IOStar
+
+  Connecting the computational monad to the specification monad using
+  a monad morphism. **)
 let rec theta #a (m:io a) : hist a =
   match m with
   | Return x -> hist_return x
-  | Call o args k -> hist_bind (op_wp o args) (fun r -> theta (k r))
+  | Call o args k -> hist_bind (hist_call o args) (fun r -> theta (k r))
 
 val theta_monad_morphism_ret (x:'a) :
   Lemma (theta (return x) == hist_return x)
@@ -60,20 +211,20 @@ let rec theta_monad_morphism_bind m k =
       `hist_equiv` { _ by (compute ()) }
       theta (Call o arg (fun x -> io_bind (m' x) k));
       `hist_equiv` { _ by (norm [delta_once [`%theta]; iota]) }
-      hist_bind (op_wp o arg) (fun r -> theta (io_bind (m' r) k));
+      hist_bind (hist_call o arg) (fun r -> theta (io_bind (m' r) k));
       `hist_equiv` {
         introduce forall r. theta (io_bind (m' r) k) `hist_equiv` hist_bind (theta (m' r)) (fun x -> theta (k x)) with begin
           theta_monad_morphism_bind (m' r) k
         end;
-        lem_hist_bind_equiv (op_wp o arg) (op_wp o arg) (fun r -> theta (io_bind (m' r) k)) (fun r -> hist_bind (theta (m' r)) (fun x -> theta (k x)))
+        lem_hist_bind_equiv (hist_call o arg) (hist_call o arg) (fun r -> theta (io_bind (m' r) k)) (fun r -> hist_bind (theta (m' r)) (fun x -> theta (k x)))
        }
-      hist_bind (op_wp o arg) (fun r -> hist_bind (theta (m' r)) (fun x -> theta (k x)));
-      `hist_equiv` { lemma_hist_bind_associativity (op_wp o arg) (fun r -> theta (m' r)) (fun x -> theta (k x)) }
-      hist_bind (hist_bind (op_wp o arg) (fun r -> theta (m' r))) (fun x -> theta (k x));
+      hist_bind (hist_call o arg) (fun r -> hist_bind (theta (m' r)) (fun x -> theta (k x)));
+      `hist_equiv` { lemma_hist_bind_associativity (hist_call o arg) (fun r -> theta (m' r)) (fun x -> theta (k x)) }
+      hist_bind (hist_bind (hist_call o arg) (fun r -> theta (m' r))) (fun x -> theta (k x));
       `hist_equiv` {
         assert (hist_equiv
           (hist_bind (theta (Call o arg m')) (fun x -> theta (k x)))
-          (hist_bind (hist_bind (op_wp o arg) (fun r -> theta (m' r))) (fun x -> theta (k x)))
+          (hist_bind (hist_bind (hist_call o arg) (fun r -> theta (m' r))) (fun x -> theta (k x)))
         ) by (norm [delta_once [`%theta]; zeta; iota];
           apply_lemma (`lem_hist_equiv_reflexive)) }
       hist_bind (theta (Call o arg m')) (fun x -> theta (k x));
@@ -93,19 +244,19 @@ let io_bind_equivalence (#a #b:Type) (k k':a -> io b) (m:io a) :
       `hist_equiv` { theta_monad_morphism_bind (Call o arg m') k }
       hist_bind (theta (Call o arg m')) (fun x -> theta (k x));
       `hist_equiv` { _ by (norm [delta_once [`%theta]; zeta;iota]) }
-      hist_bind (hist_bind (op_wp o arg) (fun r -> theta (m' r))) (fun x -> theta (k x));
-      `hist_equiv` { lemma_hist_bind_associativity (op_wp o arg) (fun r -> theta (m' r)) (fun x -> theta (k x)) }
-      hist_bind (op_wp o arg) (fun r -> hist_bind (theta (m' r)) (fun x -> theta (k x)));
+      hist_bind (hist_bind (hist_call o arg) (fun r -> theta (m' r))) (fun x -> theta (k x));
+      `hist_equiv` { lemma_hist_bind_associativity (hist_call o arg) (fun r -> theta (m' r)) (fun x -> theta (k x)) }
+      hist_bind (hist_call o arg) (fun r -> hist_bind (theta (m' r)) (fun x -> theta (k x)));
       `hist_equiv` {
-        lem_hist_bind_equiv (op_wp o arg) (op_wp o arg) (fun r -> hist_bind (theta (m' r)) (fun x -> theta (k x))) (fun r -> hist_bind (theta (m' r)) (fun x -> theta (k' x)))
+        lem_hist_bind_equiv (hist_call o arg) (hist_call o arg) (fun r -> hist_bind (theta (m' r)) (fun x -> theta (k x))) (fun r -> hist_bind (theta (m' r)) (fun x -> theta (k' x)))
       }
-      hist_bind (op_wp o arg) (fun r -> hist_bind (theta (m' r)) (fun x -> theta (k' x)));
-      `hist_equiv` { lemma_hist_bind_associativity (op_wp o arg) (fun r -> theta (m' r)) (fun x -> theta (k' x)) }
-      hist_bind (hist_bind (op_wp o arg) (fun r -> theta (m' r))) (fun x -> theta (k' x));
+      hist_bind (hist_call o arg) (fun r -> hist_bind (theta (m' r)) (fun x -> theta (k' x)));
+      `hist_equiv` { lemma_hist_bind_associativity (hist_call o arg) (fun r -> theta (m' r)) (fun x -> theta (k' x)) }
+      hist_bind (hist_bind (hist_call o arg) (fun r -> theta (m' r))) (fun x -> theta (k' x));
       `hist_equiv` {
         assert (hist_equiv
           (hist_bind (theta (Call o arg m')) (fun x -> theta (k' x)))
-          (hist_bind (hist_bind (op_wp o arg) (fun r -> theta (m' r))) (fun x -> theta (k' x)))
+          (hist_bind (hist_bind (hist_call o arg) (fun r -> theta (m' r))) (fun x -> theta (k' x)))
         ) by (norm [delta_once [`%theta]; zeta; iota];
           apply_lemma (`lem_hist_equiv_reflexive))
        }
@@ -171,7 +322,7 @@ val lem_thetaP_call (o:io_ops) (args:io_args o) (res:io_res o args) (h:history) 
 let lem_thetaP_call o args res h =
   introduce forall (p:hist_post h (io_res o args)). (theta (io_call o args)) h p ==> p [op_to_ev o args res] res with begin
     introduce (theta (io_call o args)) h p ==> p [op_to_ev o args res] res with _. begin
-      assert ((hist_bind (op_wp o args) (fun (r:io_res o args) -> theta (Return r))) h p ==>
+      assert ((hist_bind (hist_call o args) (fun (r:io_res o args) -> theta (Return r))) h p ==>
               (hist_bind (to_hist (fun h_ -> io_pre h_ o args) (fun h_ res_ lt_ -> io_post h_ o args res_ /\ lt_ == [op_to_ev o args res_])) (fun (r:io_res o args) -> theta (Return r))) h p) by (compute ());
       eliminate forall (lt':local_trace h) (r':io_res o args). lt' == [op_to_ev o args r'] ==>
         (theta (Return r')) (h++lt') (fun (lt'':local_trace (h++lt')) (r'':io_res o args) -> p (lt' @ lt'') r'')
